Add files via upload

Verif_swapsynth.v
@@ -38,8 +38,31 @@ Definition swapskip_spec : ident * funspec :=
     (*SEP(emp)*)
     SEP (data_at sh1 tint (Vint (Int.repr a)) x; data_at sh2 tint (Vint (Int.repr b)) y).
 
+  Search Int.repr.  
 
-Definition Gprog := [swapskip_spec; swap_spec].
+(*math - x is assigned to y + 1*)
+Definition swapmath_spec : ident * funspec :=
+  DECLARE _swapmath
+   WITH x: val, y: val, sh1 : share, sh2 : share, a : Z, b : Z
+   PRE [ tptr tint, tptr tint ]
+    PROP  (readable_share sh1; writable_share sh2; 
+    Int.min_signed <= Int.signed (Int.repr a) + Int.signed (Int.repr 1) <= Int.max_signed)
+    (*LOCAL (temp _x x; temp _y y)*)
+    PARAMS (x; y)
+    (*SEP(emp)*)
+    SEP (data_at sh1 tint (Vint (Int.repr a)) x; data_at sh2 tint (Vint (Int.repr b)) y)
+   POST [ tvoid ]
+    PROP () RETURN ()
+    (*SEP(emp)*)
+    SEP (data_at sh1 tint (Vint (Int.repr a)) x; data_at sh2 tint (Vint (Int.repr (a + 1))) y).
+
+Definition Gprog := [swapskip_spec; swap_spec; swapmath_spec].
+
+Lemma swapmathSynth: semax_body Vprog Gprog f_swapmath swapmath_spec.
+Proof.
+  start_function. fastforward. entailer!.
+Qed. 
+
 (*auxiliary start function 1: the function specific lemmas are commented out*)
 Ltac start_aux1 := 
   (*leaf_function;*)
@@ -215,6 +238,7 @@ Local Open Scope clight_scope.
 
 Definition _a2 : ident := $"a2".
 Definition _b2 : ident := $"b2".
+Definition _default : ident := $"default".
 (*generic body of swap with temporary variables*)
 Definition f_swap (s : statement) := {|
   fn_return := tvoid;
@@ -224,36 +248,197 @@ Definition f_swap (s : statement) := {|
   fn_temps := ((_a2, tint) :: (_b2, tint) :: nil);
   fn_body := s
 |}.
-      
+
+
+Ltac start_functionaux := start_aux1; start_aux2; start_aux3.
+
+(*all the maps*)
+Definition total_map (A : Type) := string -> A.
+(*empty maps to nil, as they are total maps*)
+Definition map_empty {A : Type} (v : A) : total_map A := (fun _ => v).
+(*update function*)
+Definition map_update {A : Type} (m : total_map A) (x : string) (v : A) := fun x' => if String.eqb x x' then v else m x'.
+(*check if an element belongs to a map*)
+(*Define ident map (string to ident) with default as the default element*)
+Definition id_map := map_update (map_update (map_update (map_update (map_empty default) "_x" _x) "_y" _y) "_a2" _a2) "_b2" _b2.
+(*Define variable (given + ghost) to identifier string*)
+Definition var_map := map_update (map_update (map_empty "nil") "x" "_x") "y" "_y".
+(*map identifiers of temp. variables to variables*)
+Definition ident_map := map_update (map_update (map_empty "nil") "_x" "x") "_y" "y".
+(*Map for precc.*)
+Definition precc_map := map_update (map_update (map_empty "nil") "x" "a") "y" "b".
+(*Map for postc.*)
+Definition postc_map := map_update (map_update (map_empty "nil") "x" "b") "y" "a".
+(*Algorithm: 
+ 1. Map : Precc. Map : Postc.
+ 2. Check: for every variable: if precc. maps to a ghost variable and not identifier -> read the variable into identifier
+ 3. Once all reading is done: Check that all precc. variables point to identifiers -> check for write
+ 4. Pre and Post same -> Exit
+*)
+Check (Sset (id_map (precc_map "x")) (Ederef (Etempvar (id_map (var_map "x")) (tptr tint)) tint)). 
+Check (Sset _a2 (Ederef (Etempvar _x (tptr tint)) tint)).
+
+Definition conc (s : string) := append (append "_" s) "2". (*used for variable names*)
+
+Definition vars := ["x";"y"].
+(*(String.eqb (ident_map (precc_map "x")) "nil").*)
+(*v1 : a; v2 : _a2 : returns new postcondition map*)
+Fixpoint updMap (varin : list string) (v1 v2 : string) (post_mcmap : total_map string) :=
+  match varin with
+  | nil => post_mcmap
+  | h :: t => if String.eqb (post_mcmap h) v1 then (updMap t v1 v2 (map_update post_mcmap h v2)) 
+              else (updMap t v1 v2 post_mcmap)
+  end. 
+
+(*read: checks for a variable if read is applicable and does updates to the maps acco*)
+Definition read_identmap (x : string) := 
+  let v := (precc_map x) in (if (String.eqb (ident_map v) "nil") then 
+  (let iden := conc v in  
+   let idmp1 := map_update ident_map iden v in 
+   let idpmp1 := map_update precc_map x iden in updMap vars v iden postc_map  
+   )    
+else ident_map).
+
+
+(*required for read - first update is to identity map*)
+Definition upd_ident (idmap : total_map string) (x v : string) := 
+  let iden := conc v in map_update idmap iden v.
+
+(*required for read - second update is to precc. map*)
+Definition upd_premap (pre_map : total_map string) (x iden : string) := 
+  map_update pre_map x iden.
+
+(*required for read - third update is for postc. map*)
+Definition upd_postmap (post_map : total_map string) (v iden : string) := 
+  updMap vars v iden post_map.
+
+
+(*write map: for a variable; check if its pre and postc. are both identifiers and both different identifiers
+map the pre id. to post*)
+Definition write_identmap (iden_map prec_map post_map : total_map string) (x : string) := 
+  let v1 := (prec_map x) in 
+  let v2 := (post_map x) in 
+  if (String.eqb (iden_map v1) "nil") then prec_map (*Read needs to happen*) 
+  else if (String.eqb (iden_map v2) "nil") then prec_map  (*Read needs to happen*)
+  else if (String.eqb v1 v2) then prec_map (*both are equal: frame*)
+  else map_update prec_map x v2 (*update precc_map for x to point to v2*)
+.
+
+
+Fixpoint readSynth (iden_map prec_map post_map : total_map string) (l : list string) :=
+  match l with 
+  | nil => (iden_map, (prec_map, post_map))
+  | h :: t => let v := (prec_map h) in (if (String.eqb (iden_map v) "nil") then 
+              (let iden := conc v in  
+              let idmp := map_update iden_map iden v in 
+              let idprmp := map_update prec_map h iden in 
+              let idpomp := updMap vars v iden post_map in 
+              readSynth idmp idprmp idpomp t  
+              )    
+             else readSynth iden_map prec_map post_map t)
+  end.
+
+Fixpoint writeSynth (iden_map prec_map post_map : total_map string) (l : list string) :=
+  match l with
+  | nil => prec_map (*only prec. map can change for write*)
+  | h :: t => writeSynth iden_map (write_identmap iden_map prec_map post_map h) post_map t
+end. 
+
+Definition readRes := readSynth ident_map precc_map postc_map vars.
+(*x,_a2,_x : readtac x _a2 _x*)
+Ltac readtac v idG idT  :=
+  match goal with
+  | |- semax _ (PROPx _ (LOCALx (temp ?t ?a :: _) (SEPx ((data_at ?sh tint ?a v) ::  _)))) _ _ => simpl
+  | |- semax _ (PROPx _ (LOCALx (temp ?t ?a :: _) (SEPx (_ ++ (data_at ?sh tint ?a v) ::  _)))) _ _ => simpl
+  | |- semax _ (PROPx _ (LOCALx (temp ?t ?a :: _) (SEPx (_ ++ [data_at ?sh tint ?a v])))) _ _ => simpl
+  | |- semax _ (PROPx _ (LOCALx (_ ++ temp ?t ?a :: _) (SEPx ((data_at ?sh tint ?a v) ::  _)))) _ _ => simpl
+  | |- semax _ (PROPx _ (LOCALx (_ ++ temp ?t ?a :: _) (SEPx (_ ++ (data_at ?sh tint ?a v) ::  _)))) _ _ => simpl
+  | |- semax _ (PROPx _ (LOCALx (_ ++ temp ?t ?a :: _) (SEPx (_ ++ [data_at ?sh tint ?a v])))) _ _ => simpl
+  | |- semax _ (PROPx _ (LOCALx (_ ++ [temp ?t ?a]) (SEPx ((data_at ?sh tint ?a v) ::  _)))) _ _ => simpl
+  | |- semax _ (PROPx _ (LOCALx (_ ++ [temp ?t ?a]) (SEPx (_ ++ (data_at ?sh tint ?a v) ::  _)))) _ _ => simpl
+  | |- semax _ (PROPx _ (LOCALx (_ ++ [temp ?t ?a]) (SEPx (_ ++ [data_at ?sh tint ?a v])))) _ _ => simpl
+  | |- semax _ (PROPx _ (LOCALx ?L (SEPx ((data_at ?sh tint ?a v) ::  _)))) _ _ => eapply semax_seq' with (c1 := (Sset idG (Ederef (Etempvar idT (tptr tint)) tint))) (*read*)
+  | |- semax _ (PROPx _ (LOCALx ?L (SEPx (_ ++ (data_at ?sh tint ?a v) ::  _)))) _ _ => eapply semax_seq' with (c1 := (Sset idG (Ederef (Etempvar idT (tptr tint)) tint))) (*read*)
+  | |- semax _ (PROPx _ (LOCALx ?L (SEPx (_ ++ [data_at ?sh tint ?a v])))) _ _ => eapply semax_seq' with (c1 := (Sset idG (Ederef (Etempvar idT (tptr tint)) tint))) (*read*)
+  end.
+
+(*x _x*)
+Ltac writetac v idV := 
+  match goal with 
+  | |- semax _ (PROPx _ (LOCALx (temp ?idt ?idv' :: _) (SEPx ((data_at ?sh tint ?idv v) ::  _)))) _ 
+        (normal_ret_assert (PROPx _ (LOCALx _ (SEPx ((data_at ?sh tint ?idv' v) ::  _)))) * _) => eapply semax_seq' with (c1 := (Sassign (Ederef (Etempvar idV (tptr tint)) tint) (Etempvar idt tint)))
+  | |- semax _ _ _ _ => simpl
+  end.
+
+
+
+
+Lemma body_swapsynthesisLtacs: exists s, semax_body Vprog Gprog (f_swap s)  swap_spec.
+Proof.
+  eexists. start_functionaux.
+  (*ltac read:  
+    F, F (D)
+    F, M (D)
+    F, L (D)
+  ——————————
+    M, F (D)
+    M, M (D)
+    M, L (D)
+  ———————————
+    L, F (D)
+    L, M (D)
+    L, L (D)*)
+    readtac x _a2 _x. apply semax_later_trivial. load_tac. simpl.
+    (*readtac y _b2 _y.*) 
+    eapply semax_seq' with (c1 := (Sset _b2 (Ederef (Etempvar _y (tptr tint)) tint))). apply semax_later_trivial. load_tac. simpl.
+    (*write - unfold*)
+Admitted.
+
+Lemma body_swapsynthesisRules: exists s, semax_body Vprog Gprog (f_swap s)  swap_spec.
+Proof.
+  eexists. start_functionaux.
+  (*check if read x is possible*)
+  Definition readResult := readSynth ident_map precc_map postc_map vars.
+  Definition pread_idmap := fst readResult.
+  Definition pre_rmap := fst (snd readResult).
+  Definition post_rmap := snd (snd readResult).
+  (*Set commands after read*)
+  (*Check precc. x -> _a2; get identifer -> idmap (_a2); var_map *)
+  (*first read*)
+  eapply semax_seq' with (c1 := ((Sset (id_map (pre_rmap "x")) (Ederef (Etempvar (id_map (var_map "x")) (tptr tint)) tint)))).
+  apply semax_later_trivial. load_tac. simpl.
+  (*second read*)
+  eapply semax_seq' with (c1 := ((Sset (id_map (pre_rmap "y")) (Ederef (Etempvar (id_map (var_map "y")) (tptr tint)) tint)))).
+  apply semax_later_trivial. load_tac. simpl.
+  (*write*)
+  Definition pre_writemap := writeSynth pread_idmap pre_rmap post_rmap vars.
+  eapply semax_seq' with (c1 := (Sassign (Ederef (Etempvar (id_map (var_map "x")) (tptr tint)) tint) (Etempvar (id_map (pre_writemap "x")) tint))).
+  apply semax_later_trivial. store_tac. simpl. 
+  (*write second*)
+  eapply semax_seq' with (c1 := (Sassign (Ederef (Etempvar (id_map (var_map "y")) (tptr tint)) tint) (Etempvar (id_map (pre_writemap "y")) tint)))(c2 := Sskip).
+  apply semax_later_trivial. store_tac. simpl. 
+  simpl. forward. entailer!.
+Qed.
+ 
+
+(*rules: Pre and Post -> decide*)
 (*swap synthesis*)
 Lemma body_swapfullsynthesis: exists s, semax_body Vprog Gprog (f_swap s)  swap_spec.
 Proof.
-  eexists. start_aux1; start_aux2; start_aux3.
+  eexists. start_functionaux.
   (*copy swap synthesis*)
   (*read*)
-  eapply semax_seq' with (c1 := (Sset _a2 (Ederef (Etempvar _x (tptr tint)) tint))). 
-  apply semax_later_trivial. load_tac. simpl.
+  eapply semax_seq' with (c1 := (Sset _a2 (Ederef (Etempvar (id_map "_x") (tptr tint)) tint))).
+  apply semax_later_trivial. load_tac. simpl. 
   (*second read*)
-  eapply semax_seq' with (c1 := (Sset _b2 (Ederef (Etempvar _y (tptr tint)) tint))).
+  eapply semax_seq' with (c1 := (Sset _b2 (Ederef (Etempvar (id_map "_y") (tptr tint)) tint))).
   apply semax_later_trivial. load_tac. simpl.
   (*first write*)
-  eapply semax_seq' with (c1 := (Sassign (Ederef (Etempvar _y (tptr tint)) tint) (Etempvar _a2 tint))).
+  eapply semax_seq' with (c1 := (Sassign (Ederef (Etempvar (id_map "_y") (tptr tint)) tint) (Etempvar _a2 tint))).
   apply semax_later_trivial. store_tac. simpl.
   (*second write*)
-  eapply semax_seq' with (c1 := (Sassign (Ederef (Etempvar _x (tptr tint)) tint) (Etempvar _b2 tint)))(c2 := Sskip).
-  apply semax_later_trivial. store_tac. simpl.
-  (*Skip*)
-  unfold POSTCONDITION. unfold abbreviate.
-  unfold stackframe_of. simpl map. rewrite fold_right_nil. 
-  rewrite sepcon_emp. simpl.
-  eapply semax_post. 5:{ eapply semax_skip. }
-  apply derives_ENTAIL. simpl. intros.  entailer!.   
-  eapply drop_LOCAL'' with (n := O). eapply drop_LOCAL'' with (n := O).
-  eapply drop_LOCAL'' with (n := O). eapply drop_LOCAL'' with (n := O). simpl. 
-  intros. entailer!.
-  apply derives_ENTAIL.
-  simpl. intros. entailer!.
-  simpl. intros. entailer!. simpl. intros. entailer!. 
+  eapply semax_seq' with (c1 := (Sassign (Ederef (Etempvar (id_map "_x") (tptr tint)) tint) (Etempvar _b2 tint)))(c2 := Sskip).
+  apply semax_later_trivial. store_tac. simpl. forward. entailer!.
 Qed.
 
 
